README.md
@@ -1,0 +1,11 @@
+# Haskelite-coq
+
+Proving Haskelite's big-step and small-step semantics equivalent.
+
+## Building
+
+Run the following command:
+
+```bash
+dune build
+```
